Generated/erc20shim/ERC20Shim/fun_spendAllowance_user.lean
@@ -22,24 +22,22 @@ def A_fun_spendAllowance  (var_owner var_spender var_value : Literal) (s₀ s₉
   s₉.isOk ∧
   (s₀.evm.isEVMState → s₉.evm.isEVMState) ∧
   (
-    ∀ {erc20}, (IsERC20 erc20 s₀ ∧ s₀.evm.isEVMState ∧ s₀.evm.reverted = false) →
+    ∀ {erc20}, (IsERC20 erc20 s₀ ∧ s₀.evm.isEVMState) →
     let currentAllowance := (erc20.allowances.lookup (owner_addr, spender_addr)).getD 0
     -- Case: spendAllowance succeeds
     (
         let allowances := update_allowances erc20 owner_addr spender_addr transfer_value
         IsERC20 ({ erc20 with allowances }) s₉ ∧
         preservesEvm s₀ s₉ ∧
-        s₉.evm.hash_collision = false ∧
-        s₉.evm.reverted = false ∧
-        s₉.store = s₀.store
+        s₉.store = s₀.store ∧
+        s₉.evm.reverted = false
     )
     ∨
     -- Case: spendAllowance fails
     (
       IsERC20 erc20 s₉ ∧
       preservesEvm s₀ s₉ ∧
-      s₉.evm.hash_collision = false ∧
-      s₉.evm.reverted = true ∧
+      s₉ = s₀.setRevert ∧
       currentAllowance < transfer_value
     )
     -- Case: Hash collision
